more network_util

theories/aneris_lang/lib/network_util.v
@@ -27,6 +27,16 @@ Definition receivefrom_all : val :=
     else "recv" "n" in
   list_fold  (λ: "acc" "n", list_append "acc" ["recv" "n"]) [] "nodes".
 
+Definition wait_receivefrom_all : val :=
+  λ: "socket" "nodes" "test",
+  letrec: "recv" "n" :=
+    let: "msg" := unSOME (ReceiveFrom "socket") in
+    let: "sender" := Snd "msg" in
+    let: "m" := Fst "msg" in
+    if: ("sender" = "n") && ("test" "m") then "m"
+    else "recv" "n" in
+  list_fold  (λ: "acc" "n", list_append "acc" ["recv" "n"]) [] "nodes".
+
 Import Network.
 
 Section library.
@@ -49,10 +59,11 @@ Section library.
         a @ φ ⤳# (R, T) }}}
       receivefrom_all #(LitSocket h) ns @[ip]
     {{{ vs msgs R', RET vs;
-        h ↪[ip] s
-          ∗ a @ φ ⤳# (R', T)
-          ∗ ⌜is_list (map (λ m, #(m_body m)) msgs) vs⌝
-          ∗ [∗ list] n ∈ nodes, (∃ m, ⌜m ∈ msgs⌝ ∗ ⌜m_sender m = n⌝ ∗ φ m) }}}.
+        h ↪[ip] s ∗
+        a @ φ ⤳# (R', T) ∗
+        ⌜length nodes = length msgs⌝ ∗
+        ⌜is_list (map (λ m, #(m_body m)) msgs) vs⌝ ∗
+        [∗ list] i↦n ∈ nodes, ∃ m, ⌜msgs !! i = Some m⌝ ∗ ⌜m_sender m = n⌝ ∗ φ m }}}.
   Proof.
     iIntros (Hip ?? Φ) "(Hns & Hh & #Hφ & Ha) HΦ".
     rewrite /receivefrom_all. wp_pures.
@@ -60,15 +71,16 @@ Section library.
                 (λ (nodes' : list socket_address) (acc : val), ∃ msgs R,
                     h ↪[ip] s ∗ a @ φ ⤳# (R, T) ∗
                       ⌜is_list (map (λ m, #(m_body m)) msgs) acc⌝ ∗
-                      [∗ list] n ∈ nodes', (∃ m, ⌜m ∈ msgs⌝ ∗ ⌜m_sender m = n⌝ ∗ φ m))%I
-                (λ n, True)%I
-                (λ n, True)%I _ _ nodes [] with "[] [$Hns Hh Ha]").
+                      ⌜length nodes' = length msgs⌝ ∗
+                      [∗ list] i↦n ∈ nodes', (∃ m, ⌜msgs !! i = Some m⌝ ∗
+                                                   ⌜m_sender m = n⌝ ∗ φ m))%I
+                (λ n, True)%I (λ n, True)%I _ _ nodes [] with "[] [$Hns Hh Ha]").
     - iIntros (n acc lacc lrem Ψ) "!# (% & Hmsgs & _) HΨ".
       do 3 wp_pure _.
       wp_bind (((rec: "recv" _ := _)%V _))%E.
       iLöb as "IH".
       wp_pures.
-      iDestruct "Hmsgs" as (msgs R') "(Hh & Ha & %Hacc & Hnodes)".
+      iDestruct "Hmsgs" as (msgs R') "(Hh & Ha & %Hacc & %Hlength & Hnodes)".
       wp_apply (aneris_wp_receivefrom_nodup with "[$Hh $Ha $Hφ]"); [done..|].
       iIntros (m) "(Hh & Ha & Hm)".
       wp_apply wp_unSOME; [done|]; iIntros "_".
@@ -84,17 +96,21 @@ Section library.
         iSplit.
         { rewrite map_app //. }
         rewrite big_sepL_app big_sepL_singleton.
+        iSplit.
+        { iPureIntro. rewrite !app_length Hlength //. }
         iSplitL "Hnodes".
         { iApply (big_sepL_impl with "Hnodes").
           iIntros "!#" (???).
           iDestruct 1 as (?) "(% & % & ?)".
           iExists _. iFrame. simplify_eq.
           iSplit; [|done].
-          iPureIntro; set_solver. }
+          iPureIntro.
+          by apply lookup_app_l_Some. }
         iExists m. iFrame.
         inversion_clear Heq.
         iSplit; [|done].
-        iPureIntro; set_solver.
+        iPureIntro.
+        rewrite Hlength -plus_n_O lookup_app_r // -minus_diag_reverse //.
       + wp_if.
         iApply ("IH" with "[-HΨ]").
         { iExists _, _. by iFrame. }
@@ -104,13 +120,101 @@ Section library.
         iFrame. iExists _, _. by iFrame.
     - rewrite big_sepL_emp. iFrame. iExists [], R. iFrame; auto.
     - iIntros (?) "[Hmsgs _]".
-      iDestruct "Hmsgs" as (msgs R') "(Hh & Ha & %Hmsgs & Hnodes)".
+      iDestruct "Hmsgs" as (msgs R') "(Hh & Ha & %Hmsgs & % & Hnodes)".
       iApply "HΦ". by iFrame.
   Qed.
 
-  Lemma wp_sendto_all f m a h s R T ns nodes :
-    let ip := ip_of_address a in
+  Lemma wp_wait_receivefrom_all Ψ nodes φ ns h s ip a R T (fv : val) :
+    ip = ip_of_address a →
+    saddress s = Some a →
+    sblock s = true →
+    (∀ (str : string),
+      {{{ True }}}
+        fv #str @[ip]
+      {{{ (b : bool), RET #b; if b then Ψ str else True }}}) -∗
+    {{{ ⌜is_list (map (LitV ∘ LitSocketAddress) nodes) ns⌝ ∗
+        h ↪[ip] s ∗
+        a ⤇ φ ∗
+        a @ φ ⤳# (R, T) }}}
+      wait_receivefrom_all #(LitSocket h) ns fv @[ip]
+    {{{ vs msgs R', RET vs;
+        h ↪[ip] s ∗
+        a @ φ ⤳# (R', T) ∗
+        ⌜is_list (map (λ m, #(m_body m)) msgs) vs⌝ ∗
+        ⌜length nodes = length msgs⌝ ∗
+        [∗ list] i↦n ∈ nodes, ∃ m, ⌜msgs !! i = Some m⌝ ∗
+                                   ⌜m_sender m = n⌝ ∗ Ψ (m_body m) ∗ φ m }}}.
+  Proof.
+    iIntros (Hip ??) "#Hfv !#". iIntros (Φ) "(Hns & Hh & #Hφ & Ha) HΦ".
+    rewrite /wait_receivefrom_all. wp_pures.
+    wp_apply (wp_list_fold
+                (λ (nodes' : list socket_address) (acc : val), ∃ msgs R,
+                    h ↪[ip] s ∗ a @ φ ⤳# (R, T) ∗
+                    ⌜is_list (map (λ m, #(m_body m)) msgs) acc⌝ ∗
+                    ⌜length nodes' = length msgs⌝ ∗
+                    [∗ list] i↦n ∈ nodes', (∃ m, ⌜msgs !! i = Some m⌝ ∗
+                                                 ⌜m_sender m = n⌝ ∗ Ψ (m_body m) ∗ φ m))%I
+                (λ n, True)%I
+                (λ n, True)%I _ _ nodes [] with "[] [$Hns Hh Ha]").
+    - iIntros (n acc lacc lrem Φ') "!# (% & Hmsgs & _) HΦ'".
+      do 3 wp_pure _.
+      wp_bind (((rec: "recv" _ := _)%V _))%E.
+      iLöb as "IH".
+      wp_pures.
+      iDestruct "Hmsgs" as (msgs R') "(Hh & Ha & %Hacc & %Hlength & Hnodes)".
+      wp_apply (aneris_wp_receivefrom_nodup with "[$Hh $Ha $Hφ]"); [done..|].
+      iIntros (m) "(Hh & Ha & Hm)".
+      wp_apply wp_unSOME; [done|]; iIntros "_".
+      wp_pures.
+      case_bool_decide as Heq.
+      + wp_pures.
+        wp_apply "Hfv"; [done|].
+        iIntros ([]) "Hb".
+        * wp_if.  wp_apply wp_list_singleton; [done|].
+          iIntros (??).
+          wp_apply wp_list_append; [done|].
+          iIntros (??). iApply "HΦ'". iSplit; [|done].
+          iExists (msgs ++ [m]), _. iFrame.
+          iSplit.
+          { rewrite map_app //. }
+          rewrite big_sepL_app big_sepL_singleton.
+          iSplit.
+          { iPureIntro. rewrite !app_length Hlength //. }
+          iSplitL "Hnodes".
+          { iApply (big_sepL_impl with "Hnodes").
+            iIntros "!#" (???).
+            iDestruct 1 as (?) "(% & % & ?)".
+            iExists _. iFrame. simplify_eq.
+            iSplit; [|done].
+            iPureIntro; by apply lookup_app_l_Some. }
+          iExists m. iFrame.
+          inversion_clear Heq.
+          iSplit; [|done].
+          iPureIntro.
+          rewrite Hlength -plus_n_O lookup_app_r // -minus_diag_reverse //.
+        * wp_if.
+          iApply ("IH" with "[-HΦ']").
+          { iExists _, _. by iFrame. }
+          iIntros (?) "[Hmsgs _]".
+          iDestruct "Hmsgs" as (msgs' R'') "(Hh & Ha & %Hmsgs' & Hnodes)".
+          iApply "HΦ'".
+          iFrame. iExists _, _. by iFrame.
+      + do 2 wp_if.
+        iApply ("IH" with "[-HΦ']").
+        { iExists _, _. by iFrame. }
+        iIntros (?) "[Hmsgs _]".
+        iDestruct "Hmsgs" as (msgs' R'') "(Hh & Ha & %Hmsgs' & %Hlength' & Hnodes)".
+        iApply "HΦ'".
+        iFrame. iExists _, _. by iFrame.
+    - rewrite big_sepL_emp. iFrame. iExists [], R. iFrame; auto.
+    - iIntros (?) "[Hmsgs _]".
+      iDestruct "Hmsgs" as (msgs R') "(Hh & Ha & %Hmsgs & %Hlength & Hnodes)".
+      iApply "HΦ". by iFrame.
+  Qed.
+
+  Lemma wp_sendto_all f m ip a h s R T ns nodes :
     let msg n := mkMessage a n (sprotocol s) m in
+    ip = ip_of_address a →
     saddress s = Some a →
     {{{ h ↪[ip] s
           ∗ a ⤳ (R, T)
@@ -127,6 +231,32 @@ Section library.
     { iIntros (n Ψ)" !# (%Hn & [Hh Ha] & #Hφ & Hmsg) H". iDestruct "Ha" as (T') "Ha".
       wp_pures.
       wp_send "Hmsg"; [rewrite /msg //|].
+      iApply "H". iFrame. eauto. }
+    iIntros "([Hh Ha] & _)".
+    iDestruct "Ha" as (?) "Ha".
+    iApply "HΦ". iFrame.
+  Qed.
+
+  Lemma wp_sendto_all_nodup f m a h s R T ns nodes Ψ :
+    let ip := ip_of_address a in
+    let msg n := mkMessage a n (sprotocol s) m in
+    saddress s = Some a →
+    {{{ h ↪[ip] s
+          ∗ a @ Ψ ⤳# (R, T)
+          ∗ ⌜is_list (map (LitV ∘ LitSocketAddress) nodes) ns⌝
+          ∗ [∗ list] n ∈ nodes, (n ⤇ f n ∗ f n (msg n)) }}}
+      sendto_all #(LitSocket h) ns #m @[ip]
+    {{{ T', RET #(); h ↪[ip] s ∗ a @ Ψ ⤳# (R, T') }}}.
+  Proof.
+    iIntros (??? Φ) "(Hh & Ha & %Hns & Hnodes) HΦ".
+    rewrite /sendto_all. wp_pures.
+    wp_apply ((wp_list_iter (λ n, n ⤇ f n ∗ f n (msg n))
+                            (λ n, True)
+                            (h ↪[ip] s ∗ ∃ T, a @ Ψ ⤳# (R, T)) with "[] [$Hnodes $Hh Ha]")%I); [|eauto|].
+    { iIntros (n ?)" !# (%Hn & [Hh Ha] & #Hφ & Hmsg) H". iDestruct "Ha" as (T') "Ha".
+      wp_pures.
+      wp_apply (aneris_wp_send_nodup with "[$Hh $Ha $Hφ Hmsg]"); [done..|].
+      iIntros "(Hh & Ha)".
       iApply "H". iFrame. eauto. }
     iIntros "([Hh Ha] & _)".
     iDestruct "Ha" as (?) "Ha".
